@prefix IAO: <http://purl.obolibrary.org/obo/IAO_> .
@prefix adms: <http://www.w3.org/ns/adms#> .
@prefix dcterms: <http://purl.org/dc/terms/> .
@prefix linkml: <https://w3id.org/linkml/> .
@prefix owl: <http://www.w3.org/2002/07/owl#> .
@prefix pav: <http://purl.org/pav/> .
@prefix rdfs: <http://www.w3.org/2000/01/rdf-schema#> .
@prefix skos: <http://www.w3.org/2004/02/skos/core#> .
@prefix tibts: <hhttp://terminology.tib.eu/schema> .
@prefix xsd: <http://www.w3.org/2001/XMLSchema#> .

tibts:Ontology a owl:Class,
        linkml:ClassDefinition ;
    rdfs:label "Ontology" ;
    rdfs:seeAlso "schema:Ontology" ;
    rdfs:subClassOf [ a owl:Restriction ;
            owl:onClass linkml:String ;
            owl:onProperty dcterms:title ;
            owl:qualifiedCardinality 1 ],
        [ a owl:Restriction ;
            owl:maxQualifiedCardinality 1 ;
            owl:onClass linkml:String ;
            owl:onProperty dcterms:alternative ],
        [ a owl:Restriction ;
            owl:maxQualifiedCardinality 1 ;
            owl:onClass linkml:String ;
            owl:onProperty <http://purl.obolibrary.org/obo/MOD_acronym> ],
        [ a owl:Restriction ;
            owl:maxQualifiedCardinality 1 ;
            owl:onClass linkml:String ;
            owl:onProperty <http://identifiers.org/alternatePrefix> ],
        [ a owl:Restriction ;
            owl:onClass linkml:String ;
            owl:onProperty <http://example.org/UNKNOWN/vann/preferredNamespacePrefix> ;
            owl:qualifiedCardinality 1 ],
        [ a owl:Restriction ;
            owl:onClass linkml:Uriorcurie ;
            owl:onProperty <http://www.w3.org/ns/dcat#accessURL> ;
            owl:qualifiedCardinality 1 ],
        [ a owl:Restriction ;
            owl:onClass linkml:Uriorcurie ;
            owl:onProperty dcterms:license ;
            owl:qualifiedCardinality 1 ],
        tibts:OptionalMetadata,
        tibts:RecommendedMetadata,
        tibts:RequiredMetadata ;
    skos:definition "An OWL ontology." ;
    skos:exactMatch owl:Ontology ;
    skos:note "For the RDF implementation, we recommend using the URI provided here as a standard, but the URI listed under **See Also** might be used as an alternative for this class." .

tibts:SkosConceptScheme a owl:Class,
        linkml:ClassDefinition ;
    rdfs:label "SkosConceptScheme" ;
    rdfs:subClassOf [ a owl:Restriction ;
            owl:maxQualifiedCardinality 1 ;
            owl:onClass linkml:String ;
            owl:onProperty <http://identifiers.org/alternatePrefix> ],
        [ a owl:Restriction ;
            owl:maxQualifiedCardinality 1 ;
            owl:onClass linkml:String ;
            owl:onProperty <http://purl.obolibrary.org/obo/MOD_acronym> ],
        [ a owl:Restriction ;
            owl:onClass linkml:Uriorcurie ;
            owl:onProperty <http://www.w3.org/ns/dcat#accessURL> ;
            owl:qualifiedCardinality 1 ],
        [ a owl:Restriction ;
            owl:onClass linkml:String ;
            owl:onProperty <http://example.org/UNKNOWN/vann/preferredNamespacePrefix> ;
            owl:qualifiedCardinality 1 ],
        [ a owl:Restriction ;
            owl:onClass linkml:Uriorcurie ;
            owl:onProperty dcterms:license ;
            owl:qualifiedCardinality 1 ],
        [ a owl:Restriction ;
            owl:onClass linkml:String ;
            owl:onProperty dcterms:title ;
            owl:qualifiedCardinality 1 ],
        [ a owl:Restriction ;
            owl:maxQualifiedCardinality 1 ;
            owl:onClass linkml:String ;
            owl:onProperty dcterms:alternative ],
        tibts:OptionalMetadata,
        tibts:RecommendedMetadata,
        tibts:RequiredMetadata ;
    skos:definition "A SKOS vocabulary serialized in RDF using the skos:ConceptScheme" ;
    skos:exactMatch skos:ConceptScheme .

<http://terminology.tib.eu/schema> a owl:Ontology ;
    rdfs:label "Ontology-Metadata-TIB" ;
    IAO:0000700 tibts:OptionalMetadata,
        tibts:RecommendedMetadata,
        tibts:RequiredMetadata ;
    dcterms:license "https://creativecommons.org/publicdomain/zero/1.0/" ;
    dcterms:title "Ontology Metadata Schema of the TIB Terminology Service" ;
    pav:version "0.0.1" ;
    linkml:generation_date "2023-03-07T13:57:00" ;
    linkml:metamodel_version "1.7.0" ;
    linkml:source_file "ontology_metadata.yaml" ;
    linkml:source_file_date "2023-03-07T13:56:48" ;
    linkml:source_file_size 23450 .

linkml:SubsetDefinition a owl:Class ;
    rdfs:label "subset_definition" .

linkml:TypeDefinition a owl:Class ;
    rdfs:label "type_definition" .

linkml:topValue a owl:DatatypeProperty ;
    rdfs:label "value" .

<http://example.org/UNKNOWN/dcterm/description> a owl:ObjectProperty,
        linkml:SlotDefinition ;
    rdfs:label "description" ;
    rdfs:range linkml:String ;
    rdfs:seeAlso "dc:description",
        "dcterms:abstract",
        "schema:abstract",
        "schema:description",
        "skos:note" ;
    rdfs:subPropertyOf tibts:versionInformation ;
    skos:definition """The ontology should describe its own contents and scope with a few words or sentences in order to inform human users what the ontology tries to accomplish.
The description is displayed in the TIB Terminology Service ontology list and on the start page of each ontology - we therefore recommend to keep it short! For an extensive discussion about the ontology you may want to consider the publication of a traditional academic article or a detailed documentation.

This metadatum is also recommended as required by:

  * https://github.com/information-artifact-ontology/ontology-metadata/pull/106#issuecomment-1117383852
  * http://purl.obolibrary.org/meta/context.jsonld
  * https://w3id.org/mod/2.0
  * https://lov.linkeddata.es/Recommendations_Vocabulary_Design.pdf
  * https://dgarijo.github.io/Widoco/doc/bestPractices/index-en.html
  * http://ceur-ws.org/Vol-3127/#paper-15
  * https://github.com/agroportal/fairness/blob/master/doc/results/FAIR-questions.md
  * [Best Practices for Implementing FAIR Vocabularies and Ontologies on the Web ](http://dgarijo.com/papers/best_practices2020.pdf)
""" ;
    skos:exactMatch <http://example.org/UNKNOWN/dcterm/description> ;
    skos:note "For the RDF implementation, we recommend using the URI provided here as a standard, but the URI(s) listed under **See Also** might be used as alternative for this predicate." .

<http://example.org/UNKNOWN/doap/bug-database> a owl:ObjectProperty,
        linkml:SlotDefinition ;
    rdfs:label "issueTracker" ;
    rdfs:range linkml:String ;
    rdfs:seeAlso "rdfs:seeAlso" ;
    rdfs:subPropertyOf tibts:versionInformation ;
    skos:definition """Ontologies should be managed with version control software like git. Ideally, the development process of an ontology is open and takes place on platforms like GitLab.com. The ontology should point to the issue tracker of its own development environment so that others may report bugs or suggestions to the developers.

This metadatum is also recommended as required by:

  * https://github.com/information-artifact-ontology/ontology-metadata/pull/106#issuecomment-1117383852
  * http://purl.obolibrary.org/meta/context.jsonld
  * https://w3id.org/mod/2.0
  * https://github.com/owlcs/miro/blob/master/miro.md#c3-communication
  * https://github.com/agroportal/fairness/blob/master/doc/results/FAIR-questions.md
""" ;
    skos:exactMatch <http://example.org/UNKNOWN/doap/bug-database> ;
    skos:note "For the RDF implementation, we recommend using the URI provided here as a standard, but the URI(s) listed under **See Also** might be used as alternative for this predicate." .

dcterms:created a owl:ObjectProperty,
        linkml:SlotDefinition ;
    rdfs:label "created" ;
    rdfs:range linkml:String ;
    rdfs:seeAlso "dc:date",
        "dcterms:issued",
        "pav:createdOn",
        "prov:generatedAtTime",
        "schema:dateCreated",
        "schema:dateIssued",
        "schema:datePublished" ;
    rdfs:subPropertyOf tibts:versionInformation ;
    skos:definition "A property to provide the date when the ontology or a term thereof came into being." ;
    skos:exactMatch dcterms:created ;
    skos:note "For the RDF implementation, we recommend using the URI provided here as a standard, but the URI(s) listed under **See Also** might be used as alternative for this predicate." .

dcterms:creator a owl:ObjectProperty,
        linkml:SlotDefinition ;
    rdfs:label "creator" ;
    rdfs:range linkml:Uriorcurie ;
    rdfs:seeAlso "dc:creator",
        "pav:createdBy",
        "prov:wasAttributedTo",
        "schema:creator" ;
    rdfs:subPropertyOf dcterms:contributor ;
    skos:definition """The ontology should state who was or is responsible for its development. It is recommended to not only provide the creators’ names but also to link to their ORCID, ROR or Wikidata profiles if available. Using an IRI to identify the creator is a must when using the dcterms:creator predicat. For a literal representations of a creator the predicate dc:creator is recommended to be in line with DCMI specs.

This metadatum is also recommended as required by:

  * https://w3id.org/mod/2.0
  * https://lov.linkeddata.es/Recommendations_Vocabulary_Design.pdf
  * https://github.com/owlcs/miro/blob/master/miro.md#c2-development-community
  * https://dgarijo.github.io/Widoco/doc/bestPractices/index-en.html
  * [Best Practices for Implementing FAIR Vocabularies and Ontologies on the Web ](http://dgarijo.com/papers/best_practices2020.pdf)
""" ;
    skos:exactMatch dcterms:creator ;
    skos:note "For the RDF implementation, we recommend using the URI provided here as a standard, but the URI(s) listed under **See Also** might be used as alternative for this predicate." .

dcterms:isReferencedBy a owl:ObjectProperty,
        linkml:SlotDefinition ;
    rdfs:label "documentation" ;
    rdfs:range linkml:String ;
    rdfs:seeAlso "foaf:homepage" ;
    rdfs:subPropertyOf tibts:versionInformation ;
    skos:definition """To familiarize interested others with the concepts and scope of your ontology, you should consider creating some kind of documentation. A relatively easy way to do this, is to use the tool [Widoco](https://pad.gwdg.de/). It generates the documentation from the ontology and a resulting html-document can be published, for example with GitLab Pages. This auto-generated document can contain customary additions that help users to understand the ontology better.
""" ;
    skos:exactMatch dcterms:isReferencedBy ;
    skos:note "For the RDF implementation, we recommend using the URI provided here as a standard, but the URI(s) listed under **See Also** might be used as alternative for this predicate." .

dcterms:modified a owl:ObjectProperty,
        linkml:SlotDefinition ;
    rdfs:label "modificationDate" ;
    rdfs:range linkml:String ;
    rdfs:seeAlso "pav:curatedOn",
        "schema:dateModified" ;
    rdfs:subPropertyOf tibts:versionInformation ;
    skos:definition "A property to provide the date when a ressource was updated." ;
    skos:exactMatch dcterms:modified ;
    skos:note "For the RDF implementation, we recommend using the URI provided here as a standard, but the URI(s) listed under **See Also** might be used as alternative for this predicate." .

dcterms:source a owl:ObjectProperty,
        linkml:SlotDefinition ;
    rdfs:label "derivedFrom" ;
    rdfs:range linkml:String ;
    rdfs:seeAlso "dc:source",
        "pav:derivedFrom",
        "prov:wasDerivedFrom" ;
    rdfs:subPropertyOf tibts:provenanceProperty ;
    skos:definition "A property to provide one or more sources from which a ressource was derived." ;
    skos:exactMatch dcterms:source ;
    skos:note "For the RDF implementation, we recommend using the URI provided here as a standard, but the URI(s) listed under **See Also** might be used as alternative for this predicate." .

owl:imports a owl:ObjectProperty,
        linkml:SlotDefinition ;
    rdfs:label "imports" ;
    rdfs:range linkml:String ;
    rdfs:subPropertyOf tibts:versionInformation ;
    skos:definition """Version information may also be accompanied by a description about changes between one version of the ontology and its predecessor.

This metadatum is also recommended as required by:

  * https://github.com/owlcs/miro/blob/master/miro.md#e4-incorporation-of-other-ontologies
  * https://github.com/agroportal/fairness/blob/master/doc/results/FAIR-questions.md
""" ;
    skos:exactMatch owl:imports .

owl:versionIRI a owl:ObjectProperty,
        linkml:SlotDefinition ;
    rdfs:label "versionURI" ;
    rdfs:range linkml:String ;
    rdfs:seeAlso "schema:schemaVersion" ;
    rdfs:subPropertyOf tibts:versionInformation ;
    skos:definition """A version URI is a persistent identifier for a version of an ontology and is used just like its PURL to reliably retrieve a former version of an ontology. Since a PURL usually only points to the latest version of an ontology, each ontology version should additionally state its version URI.
The textual version information is usually part of a version URI of an ontology.
Here is an example from the Academic Event Ontology:
```http://purl.obolibrary.org/obo/aeon/aeon-full.owl
http://purl.obolibrary.org/obo/aeon/releases/2022-11-25/aeon-full.owl```

Here is an example from ListDB Ontology:
```https://w3id.org/listdb/onto/
https://w3id.org/listdb/onto/0.0.1```

Here is an example from the GND Ontology:
```https://d-nb.info/standards/elementset/gnd#
https://d-nb.info/standards/elementset/gnd_20221010```

This metadatum is also recommended as required by:

  * https://dgarijo.github.io/Widoco/doc/bestPractices/index-en.html
  * https://doi.org/10.1371/journal.pcbi.1009041
  * http://ceur-ws.org/Vol-3127/#paper-15
  * https://github.com/agroportal/fairness/blob/master/doc/results/FAIR-questions.md
  * [Best Practices for Implementing FAIR Vocabularies and Ontologies on the Web ](http://dgarijo.com/papers/best_practices2020.pdf)
""" ;
    skos:exactMatch owl:versionIRI ;
    skos:note "For the RDF implementation, we recommend using the URI provided here as a standard, but the URI(s) listed under **See Also** might be used as alternative for this predicate." .

owl:versionInfo a owl:ObjectProperty,
        linkml:SlotDefinition ;
    rdfs:label "versionInfo" ;
    rdfs:range linkml:String ;
    rdfs:seeAlso "pav:version",
        "schema:schemaVersion" ;
    rdfs:subPropertyOf tibts:versionInformation ;
    skos:definition """Some ontologies make use of semantic versioning and employ strings like 1.0.0 as a tag to distinguish one version of their ontology from a successor. Others employ the modification date, e.g. 2022-12-21.

This metadatum is also recommended as required by:

  * https://w3id.org/mod/2.0
  * https://lov.linkeddata.es/Recommendations_Vocabulary_Design.pdf
  * https://dgarijo.github.io/Widoco/doc/bestPractices/index-en.html
  * https://doi.org/10.1371/journal.pcbi.1009041
  * http://ceur-ws.org/Vol-3127/#paper-15
  * [Best Practices for Implementing FAIR Vocabularies and Ontologies on the Web ](http://dgarijo.com/papers/best_practices2020.pdf)
""" ;
    skos:exactMatch owl:versionInfo ;
    skos:note "For the RDF implementation, we recommend using the URI provided here as a standard, but the URI(s) listed under **See Also** might be used as alternative for this predicate." .

adms:versionNotes a owl:ObjectProperty,
        linkml:SlotDefinition ;
    rdfs:label "versionNotes" ;
    rdfs:range linkml:String ;
    rdfs:seeAlso "vann:changes" ;
    rdfs:subPropertyOf tibts:versionInformation ;
    skos:definition """Version information may also be accompanied by a description about changes between one version of the ontology and its predecessor.

This metadatum is also recommended as required by:

  * https://w3id.org/mod/2.0
  * https://lov.linkeddata.es/Recommendations_Vocabulary_Design.pdf
  * https://doi.org/10.1371/journal.pcbi.1009041
  * http://ceur-ws.org/Vol-3127/#paper-15
  * https://github.com/agroportal/fairness/blob/master/doc/results/FAIR-questions.md
""" ;
    skos:exactMatch adms:versionNotes ;
    skos:note "For the RDF implementation, we recommend using the URI provided here as a standard, but the URI(s) listed under **See Also** might be used as alternative for this predicate." .

dcterms:contributor a owl:ObjectProperty,
        linkml:SlotDefinition ;
    rdfs:label "contributor" ;
    rdfs:range linkml:Uriorcurie ;
    rdfs:seeAlso "prov:wasAttributedTo" ;
    rdfs:subPropertyOf tibts:provenanceProperty ;
    skos:definition """The ontology should state who was or is contributing to its development. It is recommended to not only provide the contributor's names but also to link to their ORCID, ROR or Wikidata profiles if available. Using an IRI to identify the creator is a must when using the dcterms:contributor predicat. For a literal representations of a creator the predicate dc:contributor is recommended to be in line with DCMI specs.

This metadatum is also recommended as required by:

  * https://w3id.org/mod/2.0
  * https://lov.linkeddata.es/Recommendations_Vocabulary_Design.pdf
  * https://github.com/owlcs/miro/blob/master/miro.md#c2-development-community
  * https://dgarijo.github.io/Widoco/doc/bestPractices/index-en.html
  * [Best Practices for Implementing FAIR Vocabularies and Ontologies on the Web ](http://dgarijo.com/papers/best_practices2020.pdf)
""" ;
    skos:exactMatch dcterms:contributor ;
    skos:note "For the RDF implementation, we recommend using the URI provided here as a standard, but the URI(s) listed under **See Also** might be used as alternative for this predicate." .

tibts:OptionalMetadata a owl:Class,
        linkml:ClassDefinition ;
    rdfs:label "OptionalMetadata" ;
    rdfs:subClassOf linkml:mixin ;
    skos:definition "A mixin that provides the optional properties needed to index an ontology or SKOS vocabulary in the TIB Terminology Service." .

tibts:RecommendedMetadata a owl:Class,
        linkml:ClassDefinition ;
    rdfs:label "RecommendedMetadata" ;
    rdfs:subClassOf [ a owl:Restriction ;
            owl:maxQualifiedCardinality 1 ;
            owl:onClass linkml:String ;
            owl:onProperty dcterms:alternative ],
        [ a owl:Restriction ;
            owl:maxQualifiedCardinality 1 ;
            owl:onClass linkml:String ;
            owl:onProperty <http://identifiers.org/alternatePrefix> ],
        linkml:mixin ;
    skos:definition "A mixin that provides the recommended properties needed to index an ontology or SKOS vocabulary in the TIB Terminology Service." .

tibts:RequiredMetadata a owl:Class,
        linkml:ClassDefinition ;
    rdfs:label "RequiredMetadata" ;
    rdfs:subClassOf [ a owl:Restriction ;
            owl:maxQualifiedCardinality 1 ;
            owl:onClass linkml:String ;
            owl:onProperty <http://purl.obolibrary.org/obo/MOD_acronym> ],
        [ a owl:Restriction ;
            owl:onClass linkml:Uriorcurie ;
            owl:onProperty dcterms:license ;
            owl:qualifiedCardinality 1 ],
        [ a owl:Restriction ;
            owl:onClass linkml:Uriorcurie ;
            owl:onProperty <http://www.w3.org/ns/dcat#accessURL> ;
            owl:qualifiedCardinality 1 ],
        [ a owl:Restriction ;
            owl:onClass linkml:String ;
            owl:onProperty <http://example.org/UNKNOWN/vann/preferredNamespacePrefix> ;
            owl:qualifiedCardinality 1 ],
        [ a owl:Restriction ;
            owl:onClass linkml:String ;
            owl:onProperty dcterms:title ;
            owl:qualifiedCardinality 1 ],
        linkml:mixin ;
    skos:definition "A mixin that provides the required properties needed to index an ontology or SKOS vocabulary in the TIB Terminology Service." .

tibts:provenanceProperty a owl:ObjectProperty,
        linkml:SlotDefinition ;
    rdfs:label "provenanceProperty" ;
    rdfs:range linkml:String ;
    skos:definition "An abstract property to group all properties that deal with provenance of a ressource." .

<http://example.org/UNKNOWN/vann/preferredNamespacePrefix> a owl:ObjectProperty,
        linkml:SlotDefinition ;
    rdfs:label "preferredPrefix" ;
    rdfs:range linkml:String ;
    rdfs:seeAlso "idot:preferredPrefix" ;
    skos:definition """The official prefix of an ontology or vocabulary namespace according to the [W3C specification](https://www.w3.org/TR/1999/REC-xml-names-19990114/#NT-NCName) (e.g. **dcterms** for [http://purl.org/dc/terms/](http://purl.org/dc/terms/).

This metadatum is also recommended as required by:

  * https://github.com/information-artifact-ontology/ontology-metadata/pull/106#issuecomment-1117383852
  * http://purl.obolibrary.org/meta/context.jsonld
  * https://w3id.org/mod/2.0
  * https://lov.linkeddata.es/Recommendations_Vocabulary_Design.pdf
  * https://dgarijo.github.io/Widoco/doc/bestPractices/index-en.html
  * https://github.com/agroportal/fairness/blob/master/doc/results/FAIR-questions.md
  * [Best Practices for Implementing FAIR Vocabularies and Ontologies on the Web ](http://dgarijo.com/papers/best_practices2020.pdf)
""" ;
    skos:exactMatch <http://example.org/UNKNOWN/vann/preferredNamespacePrefix> ;
    skos:note "For the RDF implementation, we recommend using the URI provided here as a standard, but the URI(s) listed under **See Also** might be used as alternative for this predicate.",
        "The ontology should declare its own preferred prefix. The prefix should be unique. You can check whether an ontology prefix is already in use on services like [prefix.cc](https://prefix.cc) or [bioregistry.io](https://bioregistry.io)." .

<http://identifiers.org/alternatePrefix> a owl:ObjectProperty,
        linkml:SlotDefinition ;
    rdfs:label "alternativePrefix" ;
    rdfs:range linkml:String ;
    skos:definition "A prefix of an ontology or vocabulary namespace according to the [W3C specification](https://www.w3.org/TR/1999/REC-xml-names-19990114/#NT-NCName) that is not the officially preferren one but an alternative that may be used in different contexts (e.g. **DCTERMS** or **dct** instead of the [preferredPrefix](preferredPrefix) **dcterms** for [http://purl.org/dc/terms/](http://purl.org/dc/terms/)." ;
    skos:exactMatch <http://identifiers.org/alternatePrefix> ;
    skos:note "This property is recommended to be used when there are multiple prefixes in use for a namespace, to allow resolvability of CURIEs." .

<http://purl.obolibrary.org/obo/MOD_acronym> a owl:ObjectProperty,
        linkml:SlotDefinition ;
    rdfs:label "acronym" ;
    rdfs:range linkml:String ;
    rdfs:seeAlso "http://omv.ontoware.org/2005/05/ontology#acronym" ;
    skos:definition """The ID is used as a short name for the ontology or SKOS vocabulary on the TIB Terminology Service ontology list. It can be the same string as the preferred prefix. It should be unique and not contain a hyphen.

This metadatum is also recommended as required by:

        * https://github.com/information-artifact-ontology/ontology-metadata/pull/106#issuecomment-1117383852
        * https://w3id.org/mod/2.0
        * https://github.com/agroportal/fairness/blob/master/doc/results/FAIR-questions.md
        * https://bioportal.bioontology.org/ontologies/OMV
""" ;
    skos:exactMatch <http://purl.obolibrary.org/obo/MOD_acronym> ;
    skos:note "For the RDF implementation, we recommend using the URI provided here as a standard, but the URI(s) listed under **See Also** might be used as alternative for this predicate.",
        "This property is declared only as recommended in this schema although it is technically required within the configuration of the TIB TS, as it can be derived directly from the required [preferredPrefix](preferredPrefix) if not present." .

dcterms:alternative a owl:ObjectProperty,
        linkml:SlotDefinition ;
    rdfs:label "alternativeTitle" ;
    rdfs:range linkml:String ;
    skos:definition "An alternative title or name of an ontology or SKOS vocabulary." ;
    skos:exactMatch dcterms:alternative .

dcterms:license a owl:ObjectProperty,
        linkml:SlotDefinition ;
    rdfs:label "license" ;
    rdfs:range linkml:Uriorcurie ;
    rdfs:seeAlso "http://creativecommons.org/ns#license",
        "http://dbpedia.org/ontology/license",
        "http://purl.org/dc/elements/1.1/rights",
        "http://purl.org/dc/terms/rights" ;
    skos:definition """The license of the ontology/vocabulary. Ontologies and SKOS vocabularies should refer to license documents on the web via PIDs. The license text helps others to evaluate how they may reuse the ontology/vocabulary.
Only ontologies with an open license will be published on the TIB Terminology Service.

This metadatum is also recommended as required by:

  * https://github.com/information-artifact-ontology/ontology-metadata/pull/106#issuecomment-1117383852
  * http://purl.obolibrary.org/meta/context.jsonld
  * https://w3id.org/mod/2.0
  * https://lov.linkeddata.es/Recommendations_Vocabulary_Design.pdf
  * https://dgarijo.github.io/Widoco/doc/bestPractices/index-en.html
  * https://doi.org/10.1371/journal.pcbi.1009041
  * http://ceur-ws.org/Vol-3127/#paper-15 
  * [Best Practices for Implementing FAIR Vocabularies and Ontologies on the Web ](http://dgarijo.com/papers/best_practices2020.pdf)
""" ;
    skos:exactMatch dcterms:license ;
    skos:note "For the RDF implementation, we recommend using the URI provided here as a standard, but the URI(s) listed under **See Also** might be used as alternative for this predicate." .

dcterms:title a owl:ObjectProperty,
        linkml:SlotDefinition ;
    rdfs:label "title" ;
    rdfs:range linkml:String ;
    rdfs:seeAlso "dc:title",
        "schema:name" ;
    skos:definition """The title or name of an ontology or SKOS vocabulary.

This metadatum is also recommended as required by:

  * https://github.com/information-artifact-ontology/ontology-metadata/pull/106#issuecomment-1117383852
  * http://purl.obolibrary.org/meta/context.jsonld
  * https://w3id.org/mod/2.0
  * https://lov.linkeddata.es/Recommendations_Vocabulary_Design.pdf
  * https://github.com/owlcs/miro/blob/master/miro.md#a1-ontology-name
  * https://dgarijo.github.io/Widoco/doc/bestPractices/index-en.html
  * [Best Practices for Implementing FAIR Vocabularies and Ontologies on the Web ](http://dgarijo.com/papers/best_practices2020.pdf)
""" ;
    skos:exactMatch dcterms:title ;
    skos:note "For the RDF implementation, we recommend using the URI provided here as a standard, but the URI(s) listed under **See Also** might be used as alternative for this predicate." .

<http://www.w3.org/ns/dcat#accessURL> a owl:ObjectProperty,
        linkml:SlotDefinition ;
    rdfs:label "purl" ;
    rdfs:range linkml:Uriorcurie ;
    rdfs:seeAlso "owl:ontologyIRI",
        "vann:preferredNamespaceUri" ;
    skos:altLabel "namspace URI" ;
    skos:definition """The PURL of an ontology is its persistent identifier. It is usually used by within the ontology to state:
`<https://www.domain.de/myOntology> rdf:type owl:Ontology.` 
It is usually able to locate and retrieve the ontology on the world wide web, so pasting it into your web browser should retrieve a digital document. Furthermore, it is often configured to do content negotiation so that different related resources can be retrieved with the same identifier - e.g. the human-readable ontology documentation or different serializations of an ontology.        
Ontologies usually also use the PURL to identify their classes and properties, e.g. in statements like:          
    `<https://www.domain.de/myOntology#someProperty> rdf:type owl:AnnotationProperty.`
A working PURL is required to retrieve the ontology for indexing by the TIB Terminology Service.
This metadatum is also recommended by:

  * http://purl.obolibrary.org/meta/context.jsonld    
  * https://lov.linkeddata.es/Recommendations_Vocabulary_Design.pdf
  * https://dgarijo.github.io/Widoco/doc/bestPractices/index-en.html
  * https://github.com/agroportal/fairness/blob/master/doc/results/FAIR-questions.md
  * [ Best Practices for Implementing FAIR Vocabularies and Ontologies on the Web ](http://dgarijo.com/papers/best_practices2020.pdf)
""" ;
    skos:exactMatch <http://www.w3.org/ns/dcat#accessURL> ;
    skos:note "For the RDF implementation, we recommend using the URI provided here as a standard, but the URI(s) listed under **See Also** might be used as alternative for this predicate." .

linkml:ClassDefinition a owl:Class ;
    rdfs:label "class_definition" .

tibts:versionInformation a owl:ObjectProperty,
        linkml:SlotDefinition ;
    rdfs:label "versionInformation" ;
    rdfs:range linkml:String ;
    rdfs:subPropertyOf tibts:provenanceProperty ;
    skos:definition "An abstract property to group all püroperties that deal with versioning of a ressource." .

linkml:SlotDefinition a owl:Class ;
    rdfs:label "slot_definition" .


